QHLProver/Partial_State.thy
@@ -561,6 +561,20 @@ lemma cong_vec: assumes "ne = ne'" "\<And> i j. i < ne \<Longrightarrow>
   f i = f' i" shows "Matrix.vec ne f = Matrix.vec ne' f'"
   by (rule eq_vecI, insert assms, auto)
 
+lemma card_A_B_ind_in_set_A:
+     assumes a0:"A \<inter> B = {}" and a1:"finite (A::nat set)" and a2:"finite B" 
+     shows "card {i. i < length (replicate (card (A \<union> B)) 2) \<and> i \<in> ind_in_set (A \<union> B) ` A} = card A"
+proof-
+  have h1:"card (ind_in_set (A \<union> B) ` A) = card A"     
+    by (simp add: card_image ind_in_set_inj')
+  have h2:"ind_in_set (A \<union> B) ` A \<subseteq> {0..<(card A + card B)}"
+    by (metis card_Un_disjoint a0 finite_UnI a1 a2 image_mono ind_in_set_id sup_ge1)
+  have " {i. i < length (replicate (card (A \<union> B)) 2) \<and> i \<in> ind_in_set (A \<union> B) ` A} = 
+           {0..< card A + card B} \<inter>  ind_in_set (A \<union> B) ` A"
+    using h1 h2  a1 a2 a0 by (auto simp add: card_Un_disjoint)
+  then show ?thesis using h1 h2 by (simp add: Int_absorb2 Int_commute)
+qed
+
 subsection \<open>Encodings\<close>
 
 lemma digit_encode_take:
@@ -1086,6 +1100,92 @@ lemma mat_extension_unitary:
   shows "unitary (mat_extension m)"
   using assms by (simp add: mat_extension_def tensor_mat_unitary unitary_one)
 
+
+lemma scalar_tensor_1:
+  assumes a0:"d1 \<le> dim_vec v1" and a1:"d2 \<le> dim_vec v2" 
+  shows "(a::'a::field) \<cdot>\<^sub>v (tensor_vec v1 v2) = tensor_vec  (a \<cdot>\<^sub>v v1) v2"
+proof-
+  have st1len:"dim_vec (tensor_vec v1 v2) = d"
+    unfolding tensor_vec_def  
+    by (simp add: a0 state_sig.d_def)
+  then have decode_ptensor:
+    "\<And>v1 v2. \<forall>i < d. (tensor_vec v1 v2) $ i = 
+                        v1 $ (encode1 i) * v2 $ (encode2 i)"
+    by (simp add:  partial_state.tensor_vec_eval)
+  {  
+    fix i
+    assume a00:"(i::nat) < d"
+    then have "((a::'a::field) \<cdot>\<^sub>v (tensor_vec v1 v2)) $ i = 
+               a * (v1 $ (encode1 i) * 
+                   v2 $ (encode2 i))"
+      using  st1len by (simp add: decode_ptensor)
+  }
+  moreover {
+    fix i
+    assume a00:"(i::nat) < d"
+    then have d:"i<d" using a00
+      using st1len by fastforce
+    have "(tensor_vec  v1 v2) $ i =  (v1 $ (encode1 i) * v2 $ (encode2 i))"
+      using  a00 
+      by (simp add: decode_ptensor mult.assoc)
+    have "encode1 i < dim_vec v1"
+      using  d a0 partial_state.encode1_lt
+      using order_less_le_trans by blast
+    then have "(tensor_vec  (a \<cdot>\<^sub>v v1) v2) $ i = 
+               a * (v1 $ (encode1 i) * 
+                   v2 $ (encode2 i))"
+      using  a00 
+      by (simp add: decode_ptensor mult.assoc)
+  } 
+  ultimately show ?thesis
+    using st1len by auto
+qed 
+
+lemma scalar_tensor_2:
+  assumes a0:"d1 \<le> dim_vec v1" and a1:"d2 \<le> dim_vec v2" 
+  shows "(a::'a::field) \<cdot>\<^sub>v (tensor_vec v1 v2) = tensor_vec  v1 (a \<cdot>\<^sub>v v2)"
+proof-
+  have st1len:"dim_vec (tensor_vec v1 v2) = d"
+    unfolding tensor_vec_def  
+    by (simp add: a0 state_sig.d_def)
+  then have decode_ptensor:
+    "\<And>v1 v2. \<forall>i < d. (tensor_vec v1 v2) $ i = 
+                        v1 $ (encode1 i) * v2 $ (encode2 i)"
+    by (simp add:  partial_state.tensor_vec_eval)
+  {  
+    fix i
+    assume a00:"(i::nat) < d"
+    then have "((a::'a::field) \<cdot>\<^sub>v (tensor_vec v1 v2)) $ i = 
+               a * (v1 $ (encode1 i) * 
+                   v2 $ (encode2 i))"
+      using  st1len by (simp add: decode_ptensor)
+  }
+  moreover {
+    fix i
+    assume a00:"(i::nat) < d"
+    then have d:"i<d" using a00
+      using st1len by fastforce
+    have "(tensor_vec  v1 v2) $ i =  (v1 $ (encode1 i) * v2 $ (encode2 i))"
+      using  a00 
+      by (simp add: decode_ptensor mult.assoc)
+    have "encode2 i < dim_vec v2"
+      using  d a1 partial_state.encode2_lt
+      using order_less_le_trans  by blast
+    then have "(tensor_vec v1 (a \<cdot>\<^sub>v v2)) $ i = 
+               a * (v1 $ (encode1 i) * 
+                   v2 $ (encode2 i))"
+      using  a00 
+      by (simp add: decode_ptensor mult.assoc)
+  } 
+  ultimately show ?thesis
+    using st1len by auto
+qed 
+
+lemma scalar_tensor:
+  assumes a0:"d1 \<le> dim_vec v1" and a1:"d2 \<le> dim_vec v2" 
+  shows "((a::'a::field)*b) \<cdot>\<^sub>v (tensor_vec v1 v2) = tensor_vec  (a \<cdot>\<^sub>v v1) (b \<cdot>\<^sub>v v2)"
+  by (smt (verit, ccfv_SIG) a0 a1 index_smult_vec(2) scalar_tensor_1 scalar_tensor_2 smult_smult_assoc)
+
 end
 
 abbreviation "tensor_mat \<equiv> partial_state.tensor_mat"
@@ -1137,14 +1237,14 @@ subsection \<open>Partial tensor product\<close>
 text \<open>In this context, we assume two disjoint sets of variables, and define
   the tensor product of two matrices on these variables\<close>
 
-locale partial_state2 = state_sig + 
+locale partial_state2 = 
   fixes vars1 :: "nat set"
     and vars2 :: "nat set"
   assumes disjoint: "vars1 \<inter> vars2 = {}" and
-          dims_eq: "\<forall>i<length dims. dims ! i = 2" and
           finite_v1:"finite vars1" and finite_v2:"finite vars2"
 
 begin
+
 
 definition vars0 :: "nat set" where
   "vars0 = vars1 \<union> vars2"
@@ -1173,7 +1273,7 @@ lemma "finite vars1 \<Longrightarrow> finite vars2 \<Longrightarrow> vars1 \<int
 lemma dims_product:
   "d0 = d1 * d2"
   unfolding d0_def d1_def d2_def dims0_def dims1_def dims2_def vars0_def
-  using dims_eq disjoint finite_v1 finite_v2 apply auto
+  using  disjoint finite_v1 finite_v2 apply auto
   by (simp add: card_Un_disjoint power_add)  
 
 text \<open>Locations of variables in vars1 relative to vars0.
@@ -1197,7 +1297,7 @@ lemma vars1'D:
 text \<open>Main property of vars1'\<close>
 
 lemma ind_in_set_bij:
-  "bij_betw (ind_in_set vars0) ({0..<length dims} \<inter> vars0) {0..<card ({0..<length dims} \<inter> vars0)}"
+  "bij_betw (ind_in_set vars0) ({0..<length dims0} \<inter> vars0) {0..<card ({0..<length dims0} \<inter> vars0)}"
   using bij_ind_in_set_bound unfolding ind_in_set_def by auto
 
 lemma length_dims0:
@@ -1473,12 +1573,10 @@ lemma ptensor_vec_comm:
   assumes "vars1 \<inter> vars2 = {}" and  "finite vars1" and "finite vars2"
   shows "ptensor_vec  vars1 vars2 v1 v2 = ptensor_vec  vars2 vars1 v2 v1"  
 proof -
-  let ?dims = "replicate (card (vars1 \<union> vars2)) 2"
-  have "\<forall>i<length ?dims. ?dims ! i = 2"
-    by simp 
-  interpret st1: partial_state2 ?dims vars1 vars2
+ 
+  interpret st1: partial_state2 vars1 vars2
     apply unfold_locales using assms by auto
-  interpret st2: partial_state2 ?dims vars2 vars1
+  interpret st2: partial_state2  vars2 vars1
     apply unfold_locales using assms by auto
 
   have eq1: "partial_state.encode1 st1.dims0 st1.vars1' = partial_state.encode2 st2.dims0 st2.vars1'"
@@ -1503,11 +1601,10 @@ lemma ptensor_mat_comm:
   assumes "vars1 \<inter> vars2 = {}" and "finite vars1" and "finite vars2"
   shows "ptensor_mat vars1 vars2 m1 m2 = ptensor_mat vars2 vars1 m2 m1"  
 proof -
-  let ?dims = "replicate (card (vars1 \<union> vars2)) 2"
   
-  interpret st1: partial_state2 ?dims vars1 vars2
+  interpret st1: partial_state2 vars1 vars2
     apply unfold_locales using assms by auto
-  interpret st2: partial_state2 ?dims vars2 vars1
+  interpret st2: partial_state2 vars2 vars1
     apply unfold_locales using assms by auto
 
   have eq1: "partial_state.encode1 st1.dims0 st1.vars1' = partial_state.encode2 st2.dims0 st2.vars1'"
@@ -1540,13 +1637,13 @@ proof -
   have f_v1:"finite vars1" and f_v2:"finite vars2" and f_v3:"finite vars3"
     using assms
     using subset_eq_atLeast0_lessThan_finite by blast+
-  interpret a: partial_state2 ?dims vars1 vars2
+  interpret a: partial_state2  vars1 vars2
     apply unfold_locales using assms f_v1 f_v2 f_v3 by auto
-  interpret b: partial_state2 ?dims "vars1 \<union> vars2" vars3
+  interpret b: partial_state2  "vars1 \<union> vars2" vars3
     apply unfold_locales using assms f_v1 f_v2 f_v3 by auto
-  interpret c: partial_state2 ?dims vars2 vars3
+  interpret c: partial_state2  vars2 vars3
     apply unfold_locales using assms f_v1 f_v2 f_v3 by auto
-  interpret d: partial_state2 ?dims vars1 "vars2 \<union> vars3"
+  interpret d: partial_state2  vars1 "vars2 \<union> vars3"
     apply unfold_locales using assms f_v1 f_v2 f_v3 by auto
 
   have uassoc: "vars1 \<union> (vars2 \<union> vars3) = vars1 \<union> vars2 \<union> vars3"
@@ -1693,16 +1790,13 @@ lemma tensor_mat_dim:
          carrier_mat (prod_list (replicate (card (vars1 \<union> vars2)) 2)) 
                      (prod_list (replicate (card (vars1 \<union> vars2)) 2))"
 proof-
-  let ?dims = "replicate (card (vars1 \<union> vars2)) 2"
   have f_v1:"finite vars1" and f_v2:"finite vars2" 
     using assms
     using subset_eq_atLeast0_lessThan_finite by blast+
-  interpret ps2: partial_state2 ?dims vars1 vars2
+  interpret ps2: partial_state2  vars1 vars2
     apply unfold_locales using assms f_v1 f_v2  by auto
-  have "ps2.d0 = prod_list ?dims" 
-    unfolding ps2.d0_def ps2.dims0_def ps2.vars0_def by auto    
-  then show ?thesis using ps2.ptensor_mat_carrier
-    by auto                             
+  show ?thesis using ps2.ptensor_mat_carrier
+    using ps2.d0_def ps2.dims0_def ps2.vars0_def by auto
 qed
 
 lemma ptensor_mat_assoc:
@@ -1715,13 +1809,13 @@ proof -
   have f_v1:"finite vars1" and f_v2:"finite vars2" and f_v3:"finite vars3"
     using assms
     using subset_eq_atLeast0_lessThan_finite by blast+
-  interpret a: partial_state2 ?dims vars1 vars2
+  interpret a: partial_state2  vars1 vars2
     apply unfold_locales using assms f_v1 f_v2 f_v3 by auto
-  interpret b: partial_state2 ?dims "vars1 \<union> vars2" vars3
+  interpret b: partial_state2  "vars1 \<union> vars2" vars3
     apply unfold_locales using assms f_v1 f_v2 f_v3 by auto
-  interpret c: partial_state2 ?dims vars2 vars3
+  interpret c: partial_state2 vars2 vars3
     apply unfold_locales using assms f_v1 f_v2 f_v3 by auto
-  interpret d: partial_state2 ?dims vars1 "vars2 \<union> vars3"
+  interpret d: partial_state2 vars1 "vars2 \<union> vars3"
     apply unfold_locales using assms f_v1 f_v2 f_v3 by auto
 
   have uassoc: "vars1 \<union> (vars2 \<union> vars3) = vars1 \<union> vars2 \<union> vars3"
@@ -1875,17 +1969,17 @@ lemma pmat_extension_assoc:
   shows "pmat_extension vars1 (vars2 \<union> vars3) m =
          pmat_extension (vars1 \<union> vars2) vars3 (pmat_extension  vars1 vars2 m)"
 proof -
-   let ?dims = "replicate (card (vars1 \<union> vars2 \<union> vars3)) 2"
+  
    have f_v1:"finite vars1" and f_v2:"finite vars2" and f_v3:"finite vars3"
     using assms
     using subset_eq_atLeast0_lessThan_finite by blast+
-  interpret a: partial_state2 ?dims vars1 vars2
+  interpret a: partial_state2 vars1 vars2
     apply unfold_locales using assms f_v1 f_v2 f_v3 by auto
-  interpret b: partial_state2 ?dims "vars1 \<union> vars2" vars3
+  interpret b: partial_state2  "vars1 \<union> vars2" vars3
     apply unfold_locales using assms f_v1 f_v2 f_v3 by auto
-  interpret c: partial_state2 ?dims vars2 vars3
+  interpret c: partial_state2 vars2 vars3
     apply unfold_locales using assms f_v1 f_v2 f_v3 by auto
-  interpret d: partial_state2 ?dims vars1 "vars2 \<union> vars3"
+  interpret d: partial_state2 vars1 "vars2 \<union> vars3"
     apply unfold_locales using assms f_v1 f_v2 f_v3 by auto
   have "a.d2 = c.d1"
     by (simp add: c.d1_def a.d2_def c.dims1_def a.dims2_def)
@@ -1898,6 +1992,7 @@ proof -
     by (simp add: \<open>c.d0 = d.d2\<close>)
 qed
 
+value "prod_list (replicate (card ({}::(nat set))) (2::nat)) "
 
 lemma pscalar_ptensor_1:
   assumes a0:"vs1 \<inter> vs2 = {}" and a1:"finite vs1" and a2:"finite vs2" and
@@ -1907,7 +2002,7 @@ lemma pscalar_ptensor_1:
 proof-
   let ?dims = "replicate (card (vs1 \<union> vs2)) 2"
   
-  interpret st1: partial_state2 ?dims vs1 vs2
+  interpret st1: partial_state2  vs1 vs2
     apply unfold_locales using assms by auto
   have st1len:"dim_vec (ptensor_vec vs1 vs2 v1 v2) = 2^(card st1.vars0)"
     by (simp add: st1.d0_def st1.dims0_def)
@@ -1932,12 +2027,11 @@ proof-
   moreover {
     fix i
     assume a00:"(i::nat) < 2^(card st1.vars0)"
-    have d:"st1.d = 2^(card st1.vars0)"
-      unfolding st1.d_def st1.vars0_def by auto       
-    have d1:"st1.d1 =  2^card vs1"
+          
+    have d1:"st1.d1 =  2^card vs1" unfolding st1.d1_def st1.dims1_def
       by (simp add: st1.d1_def st1.dims1_def)
     have "partial_state.encode1 st1.dims0 st1.vars1' i < dim_vec v1"
-      using a00 d a3 partial_state.encode1_lt  st1.nths_vars1'
+      using a00 a3 partial_state.encode1_lt  st1.nths_vars1'
       unfolding partial_state.d1_def partial_state.dims1_def  st1.dims0_def st1.dims1_def state_sig.d_def
       apply auto
       by (metis prod_list_replicate)         
@@ -1957,55 +2051,27 @@ lemma pscalar_ptensor_2:
   assumes a0:"vs1 \<inter> vs2 = {}" and a1:"finite vs1" and a2:"finite vs2" and
   a3:"dim_vec v1 = 2^card vs1" and a4:"dim_vec v2 = 2^card vs2"
   shows "(a::'a::field) \<cdot>\<^sub>v (ptensor_vec vs1 vs2 v1 v2) =
-    ptensor_vec vs1 vs2 v1 (a \<cdot>\<^sub>v v2)"  
-proof-
-  let ?dims = "replicate (card (vs1 \<union> vs2)) 2"
-  
-  interpret st1: partial_state2 ?dims vs1 vs2
-    apply unfold_locales using assms by auto
-  have st1len:"dim_vec (ptensor_vec vs1 vs2 v1 v2) = 2^(card st1.vars0)"
-    by (simp add: st1.d0_def st1.dims0_def)
-  have decode_ptensor:"\<And>v1 v2. \<forall>i < 2^(card st1.vars0). 
-          (ptensor_vec vs1 vs2 v1 v2) $ i = 
-             v1 $ (partial_state.encode1 st1.dims0 st1.vars1' i) * 
-             v2 $ (partial_state.encode2 st1.dims0 st1.vars1' i)"
-     by (simp add: partial_state.tensor_vec_eval st1.dims0_def 
-                    st1.ptensor_vec_def state_sig.d_def)
-  {  
-    fix i
-    assume a00:"(i::nat) < 2^(card st1.vars0)"
-    then have "((a::'a::field) \<cdot>\<^sub>v (ptensor_vec vs1 vs2 v1 v2)) $ i = 
-                a * ((ptensor_vec vs1 vs2 v1 v2)$i)"
-      using st1len by (simp add:  a00)  
-    then have "((a::'a::field) \<cdot>\<^sub>v (ptensor_vec vs1 vs2 v1 v2)) $ i = 
-               a * (v1 $ (partial_state.encode1 st1.dims0 st1.vars1' i) * 
-                   v2 $ (partial_state.encode2 st1.dims0 st1.vars1' i))"
-      using  a00
-      by (simp add: decode_ptensor)
-  }
-  moreover {
-    fix i
-    assume a00:"(i::nat) < 2^(card st1.vars0)"
-    have d:"st1.d = 2^(card st1.vars0)"
-      unfolding st1.d_def st1.vars0_def by auto       
-    have d2:"st1.d2 =  2^card vs2"
-      by (simp add: st1.d2_def st1.dims2_def)
-    have "partial_state.encode2 st1.dims0 st1.vars1' i < dim_vec v2"
-      using a00 d a4 partial_state.encode2_lt  st1.nths_vars2' a0
-      unfolding partial_state.d2_def partial_state.dims2_def st1.dims0_def st1.dims2_def 
-               state_sig.d_def st1.vars0_def       
-      by (metis prod_list_replicate )         
-    then have "(a \<cdot>\<^sub>v v2) $ (partial_state.encode2 st1.dims0 st1.vars1' i) = a *(v2 $ (partial_state.encode2 st1.dims0 st1.vars1' i))"
-      by auto
-    then have "(ptensor_vec vs1 vs2 v1 (a \<cdot>\<^sub>v v2)) $ i = 
-                 a*(v1 $ (partial_state.encode1 st1.dims0 st1.vars1' i)) * 
-                   (v2 $ (partial_state.encode2 st1.dims0 st1.vars1' i))"
-      using  a00 
-      by (auto simp add: decode_ptensor)    
-      
-  } 
-  ultimately show ?thesis
-    using st1len by auto
+    ptensor_vec vs1 vs2 v1 (a \<cdot>\<^sub>v v2)"
+  by (metis a0 a1 a2 a3 a4 inf_commute pscalar_ptensor_1 ptensor_vec_comm)  
+
+lemma pscalar_ptensor:
+  assumes a0:"vs1 \<inter> vs2 = {}" and a1:"finite vs1" and a2:"finite vs2" and
+  a3:"dim_vec v1 = 2^card vs1" and a4:"dim_vec v2 = 2^card vs2"
+  shows "((a::'a::field) * b) \<cdot>\<^sub>v (ptensor_vec vs1 vs2 v1 v2) =
+    ptensor_vec vs1 vs2 (a \<cdot>\<^sub>v v1) (b \<cdot>\<^sub>v v2)"
+proof -
+  have f1: "a * b \<cdot>\<^sub>v ptensor_vec vs1 vs2 v1 v2 = a \<cdot>\<^sub>v (b \<cdot>\<^sub>v ptensor_vec vs1 vs2 v1 v2)"
+    by (simp add: smult_smult_assoc)
+  have f2: "{} = vs1 \<inter> vs2 \<and> finite vs1 \<and> finite vs2 \<and> dim_vec v1 = 2 ^ card vs1 \<and> dim_vec v2 = 2 ^ card vs2"
+    using a0 a1 a2 a3 a4 by presburger
+  have f3: "2 ^ card vs2 = dim_vec (b \<cdot>\<^sub>v v2)"
+    using a4 by fastforce
+  have f4: "b \<cdot>\<^sub>v ptensor_vec vs1 vs2 v1 v2 = ptensor_vec vs1 vs2 v1 (b \<cdot>\<^sub>v v2)"
+    using f2 by (simp add: pscalar_ptensor_2)
+  have "ptensor_vec vs1 vs2 (a \<cdot>\<^sub>v v1) (b \<cdot>\<^sub>v v2) = a \<cdot>\<^sub>v ptensor_vec vs1 vs2 v1 (b \<cdot>\<^sub>v v2)"
+    using f3 by (simp add: a0 a1 a2 a3 pscalar_ptensor_1)
+  then show ?thesis
+    using f4 f1 by presburger
 qed
 
 subsection \<open>Commands on subset of variables\<close>
